examples/TrivialMem2.v
@@ -17,5 +17,5 @@ Definition read := bmodule "read" {{
 }}.
 
 Theorem readOk : moduleOk read.
-  vcgen; abstract (sep tt).
+  vcgen; abstract (sep_auto).
 Qed.
